Introduce locale lazify
The new locale allows us to introduce abbreviations such as sample by fixing the sampling space.
It also uses a more precise depends_on predicate, since we actually care about the invariance of the
function only on the sample space.

isabelle/Utils/PMF/Utils_PMF_Lazify.thy
@@ -7,32 +7,34 @@ imports
 
 begin
 
-definition depends_on :: "('a \<Rightarrow> 'b, 'c) reader_monad \<Rightarrow> 'a set \<Rightarrow> bool"
-  where
-    "depends_on m S = (\<forall>f g. restrict f S = restrict g S \<longrightarrow> run_reader m f = run_reader m g)"
+locale lazify =
+  fixes I :: "'a set"
+  fixes d :: "'c"
+  fixes M :: "'a \<Rightarrow> 'c pmf"
+  assumes fin_I: "finite I"
+begin
+
+definition space where "space = Pi_pmf I d M"
+definition sample where "sample x = map_pmf (run_reader x) space"
+
+definition depends_on :: "('a \<Rightarrow> 'c, 'b) reader_monad \<Rightarrow> 'a set \<Rightarrow> bool"
+  where "depends_on m S =
+    (\<forall>f g. {f,g}\<subseteq>set_pmf space \<longrightarrow> (\<lambda>i\<in>S. f i) = (\<lambda>i\<in>S. g i) \<longrightarrow> run_reader m f = run_reader m g)"
 
 lemma depends_onI:
-  assumes "\<And>f g. restrict f S = restrict g S \<Longrightarrow> run_reader m f = run_reader m g"
+  assumes "\<And>f g.
+    f \<in> set_pmf space \<Longrightarrow>
+    g \<in> set_pmf space \<Longrightarrow>
+    restrict f S = restrict g S \<Longrightarrow> run_reader m f = run_reader m g"
   shows "depends_on m S"
-  using assms unfolding depends_on_def by metis
+  using assms unfolding depends_on_def by auto
 
 lemma depends_onD:
-  assumes "depends_on m S" "restrict f S = restrict g S"
+  assumes "depends_on m S"
+  assumes "f \<in> set_pmf space" "g \<in> set_pmf space"
+  assumes "restrict f S = restrict g S"
   shows "run_reader m f = run_reader m g"
   using depends_on_def assms by auto
-
-lemma depends_on_cong:
-  fixes m n :: "('a \<Rightarrow> 'b, 'c) reader_monad"
-  assumes "S = T"
-  assumes "\<And>x. run_reader m x = run_reader n x"
-  shows "depends_on m S \<longleftrightarrow> depends_on n T"
-  using assms unfolding depends_on_def by simp
-
-lemma depends_on_univ: "depends_on f UNIV"
-  unfolding depends_on_def by (simp add: restrict_UNIV)
-
-lemma depends_on_return: "depends_on (return_rd c) S"
-  unfolding depends_on_def return_rd_def by simp
 
 lemma depends_on_mono:
   assumes "depends_on m T" "T \<subseteq> S"
@@ -40,58 +42,95 @@ lemma depends_on_mono:
   using depends_onD[OF assms(1)] assms(2)
   by (intro depends_onI) (metis restrict_restrict inf.absorb_iff2)
 
+lemma depends_on_restrict:
+  "depends_on m S = depends_on m (S \<inter> I)"
+proof -
+  have a:"restrict f S = (\<lambda>i. if i \<in> (S \<inter> I) then f i else (if i \<in> S then d else undefined))"
+    if "f \<in> set_pmf space" for f
+    using that unfolding restrict_def space_def set_Pi_pmf[OF fin_I] PiE_dflt_def by auto
+
+  have "depends_on m (S \<inter> I)" if "depends_on m S"
+  proof (rule depends_onI)
+    fix f g
+    assume b:"f \<in> set_pmf space" "g \<in> set_pmf space"
+    assume c:"restrict f (S \<inter> I) = restrict g (S \<inter> I)"
+
+    hence "restrict f S = restrict g S"
+      unfolding a[OF b(1)] a[OF b(2)] by (intro ext if_cong refl) (metis restrict_apply')
+
+    thus "run_reader m f = run_reader m g"
+      using depends_onD[OF that] b by blast
+  qed
+
+  thus ?thesis using depends_on_mono by auto
+qed
+
+lemma depends_on_cong:
+  assumes "S \<inter> I = T \<inter> I"
+  assumes "\<And>x. x \<in> set_pmf space \<Longrightarrow> run_reader m x = run_reader n x"
+  shows "depends_on m S \<longleftrightarrow> depends_on n T"
+proof -
+  have "depends_on m (S \<inter> I) = depends_on n (T \<inter> I)"
+    using assms(1,2) unfolding depends_on_def by auto
+  thus ?thesis using depends_on_restrict by auto
+qed
+
+lemma depends_on_univ: "depends_on f UNIV"
+  unfolding depends_on_def by (simp add: restrict_UNIV)
+
+lemma depends_on_return: "depends_on (return_rd c) S"
+  unfolding depends_on_def return_rd_def by simp
+
 lemma depends_on_bind:
-  fixes m :: "('i \<Rightarrow> 'c, 'a) reader_monad"
-  fixes f :: "'a \<Rightarrow> ('i \<Rightarrow> 'c, 'b) reader_monad"
   assumes "depends_on m S" "\<And>x. depends_on (f (run_reader m x)) S"
   shows "depends_on (bind_rd m f) S"
 proof (rule depends_onI)
-  fix x y :: "'i \<Rightarrow> 'c"
-  assume a:"restrict x S = restrict y S"
+  fix x y :: "'a \<Rightarrow> 'c"
+  assume a: "x \<in> set_pmf space" "y \<in> set_pmf space"  "restrict x S = restrict y S"
   show "run_reader (m \<bind> f) x = run_reader (m \<bind> f) y"
     unfolding run_reader_simps depends_onD[OF assms(1) a] depends_onD[OF assms(2) a] by simp
 qed
 
 lemma depends_on_bind_eq:
-  fixes m :: "('i \<Rightarrow> 'c, 'a) reader_monad"
-  fixes f :: "'a \<Rightarrow> ('i \<Rightarrow> 'c, 'b) reader_monad"
-  assumes "\<And>w. w \<in> ran_rd m \<Longrightarrow> v \<in> ran_rd (f w) \<Longrightarrow>
+  assumes "\<And>w. w \<in> set_pmf (sample m) \<Longrightarrow> v \<in> set_pmf (sample (f w)) \<Longrightarrow>
     depends_on (map_rd ((=) w) m) S \<and> depends_on (map_rd ((=) v) (f w)) S"
   shows "depends_on (map_rd ((=) v) (bind_rd m f)) S"
 proof (rule depends_onI)
-  fix x y :: "'i \<Rightarrow> 'c"
-  assume a:"restrict x S = restrict y S"
+  fix x y :: "'a \<Rightarrow> 'c"
+  assume a: "x \<in> set_pmf space" "y \<in> set_pmf space" "restrict x S = restrict y S"
 
   let ?dep1 = "(\<lambda>w. depends_on (map_rd ((=) (run_reader m w)) m) S) "
   let ?dep2 = "(\<lambda>w. depends_on (map_rd ((=) v) (f (run_reader m w))) S)"
 
-  have b:"?dep1 w" "?dep2 w" if "run_reader (f (run_reader m w)) w = v" for w
+  have b:"?dep1 \<phi>" "?dep2 \<phi>" if "run_reader (f (run_reader m \<phi>)) \<phi> = v"
+    "\<phi> \<in> set_pmf space" for \<phi>
   proof -
-    have "v \<in> ran_rd (f (run_reader m w)) \<and> run_reader m w \<in> ran_rd m"
-      using that unfolding ran_rd_def by auto
-    thus "?dep1 w" "?dep2 w" using assms by auto
+    let ?w = "run_reader m \<phi>"
+    have "run_reader m \<phi> \<in> set_pmf (sample m) \<and> v \<in> set_pmf (sample (f ?w))"
+      using that unfolding sample_def by auto
+    thus "?dep1 \<phi>" "?dep2 \<phi>" using assms by auto
   qed
 
   have "run_reader (f (run_reader m x)) x = v \<longleftrightarrow> run_reader (f (run_reader m y)) y = v"
-    using depends_onD[OF b(1) a] depends_onD[OF b(2) a] unfolding run_reader_simps by metis
+    using a depends_onD[OF b(1) a] depends_onD[OF b(2) a] unfolding run_reader_simps by metis
   thus "run_reader (map_rd ((=) v) (m \<bind> f)) x = run_reader (map_rd ((=) v) (m \<bind> f)) y"
     by (auto simp add:run_reader_simps)
 qed
 
 lemma depends_on_map:
-  fixes f :: "('i \<Rightarrow> 'c) \<Rightarrow> 'a"
-  assumes "\<And>c1 c2. restrict c1 S = restrict c2 S \<Longrightarrow> f c1 = f c2"
+  assumes "\<And>c1 c2. c1 \<in> set_pmf space \<Longrightarrow>
+    c2 \<in> set_pmf space \<Longrightarrow> restrict c1 S = restrict c2 S \<Longrightarrow> f c1 = f c2"
   shows "depends_on (map_rd f get_rd) S"
 proof (rule depends_onI)
-  fix c1 c2 :: "'i \<Rightarrow> 'c"
-  assume "restrict c1 S = restrict c2 S"
+  fix c1 c2 :: "'a \<Rightarrow> 'c"
+  assume "c1 \<in> set_pmf space" "c2 \<in> set_pmf space" "restrict c1 S = restrict c2 S"
   hence "f c1 = f c2" by (rule assms)
   thus "run_reader (map_rd f get_rd) c1 = run_reader (map_rd f get_rd) c2"
     by (simp add:run_reader_simps)
 qed
 
-definition independent_bind
-  where "independent_bind m f = (\<forall>v. \<exists>I. depends_on (map_rd ((=) v) m) I \<and> depends_on (f v) (UNIV - I))"
+definition independent_bind where
+  "independent_bind m f = (\<forall>v. \<exists>I. depends_on (map_rd ((=) v) m) I \<and> depends_on (f v) (UNIV - I))"
 
 lemma independent_bindI:
   assumes "\<And>v. depends_on (map_rd ((=) v) m) (F v) \<and> depends_on (f v) (UNIV - (F v))"
@@ -99,123 +138,149 @@ lemma independent_bindI:
   using assms unfolding independent_bind_def by auto
 
 lemma lazify_bind:
-  fixes I d p
-  fixes m :: "('i \<Rightarrow> 'c, 'a) reader_monad"
-  fixes f :: "'a \<Rightarrow> ('i \<Rightarrow> 'c, 'b) reader_monad"
-  assumes "independent_bind m f" "finite I"
-  defines "q \<equiv> Pi_pmf I d p"
-  shows "map_pmf (run_reader (bind_rd m f)) q = bind_pmf (map_pmf (run_reader m) q) (\<lambda>x. map_pmf (run_reader (f x)) q)"
+  fixes m :: "('a \<Rightarrow> 'c, 'b) reader_monad"
+  fixes f :: "'b \<Rightarrow> ('a \<Rightarrow> 'c, 'd) reader_monad"
+  assumes "independent_bind m f"
+  shows "sample (bind_rd m f) = sample m \<bind> (\<lambda>v. sample (f v))"
     (is "?L = ?R")
 proof -
-  let ?runr = "(\<lambda>x \<phi>. run_reader x \<phi>)"
-  let ?run = "\<lambda>x. map_pmf (run_reader x) q"
+  let ?r = "\<lambda>x \<phi>. run_reader x \<phi>"
 
-  have a:"map_pmf (\<lambda>\<phi>. let v=?runr m \<phi> in (v,?runr (f v) \<phi>)) q = bind_pmf (?run m) (\<lambda>v. map_pmf (Pair v) (?run (f v)))"
+  define \<delta> where "\<delta> i = (if i \<in> I then (SOME x. x \<in> set_pmf (M i)) else d)" for i
+  have \<delta>_ran_1: "\<delta> i \<in> set_pmf (M i)" if "i \<in> I" for i
+    unfolding \<delta>_def using that set_pmf_not_empty by (auto simp:some_in_eq)
+  have \<delta>_ran_2: "\<delta> i = d" if "i \<notin> I" for i using that unfolding \<delta>_def by simp
+
+  have 0:"(\<lambda>i. if i \<in> J then f i else \<delta> i) \<in> set_pmf space"
+    if "f \<in> Pi_pmf K d M" and "J \<subseteq> K" "K \<subseteq> I" for J K f
+  proof -
+    have fin_K: "finite K" using that fin_I finite_subset by metis
+    show ?thesis using that \<delta>_ran_1 \<delta>_ran_2
+      unfolding space_def set_Pi_pmf[OF fin_I] set_Pi_pmf[OF fin_K] PiE_dflt_def by auto
+  qed
+
+  have 1:"(\<lambda>i. if i \<in> J then f i else \<delta> i) \<in> set_pmf space" if "f \<in> Pi_pmf J d M" "J \<subseteq> I" for J f
+    using that 0 by auto
+
+  have 2:"(\<lambda>i. if i \<in> J then f i else \<delta> i) \<in> set_pmf space" if "f \<in> set_pmf space" "J \<subseteq> I" for J f
+    using that 0 unfolding space_def by auto
+
+  have a:"map_pmf (\<lambda>\<phi>. let v=?r m \<phi> in (v,?r (f v) \<phi>)) space =
+    sample m \<bind> (\<lambda>v. map_pmf (Pair v) (sample (f v)))"
     (is "?L1 = ?R1")
   proof (rule pmf_eqI)
-    fix \<omega> :: "'a \<times> 'b"
-    obtain J where J_dep: "depends_on (map_rd ((=) (fst \<omega>)) m) J" "depends_on (f (fst \<omega>)) (UNIV - J)"
+    fix \<omega> :: "'b \<times> 'd"
+    obtain J where J_dep: "depends_on (map_rd ((=) (fst \<omega>)) m) J \<and> depends_on (f (fst \<omega>)) (UNIV-J)"
       using assms(1) unfolding independent_bind_def by auto
+    moreover have " I-J = (UNIV - J) \<inter> I" by blast
+    ultimately have J_dep:"depends_on (map_rd ((=) (fst \<omega>)) m) (J\<inter>I)" "depends_on (f (fst \<omega>)) (I-J)"
+      using depends_on_restrict by auto
 
-    have fins: "finite (J \<inter> I)" "finite (I - J)" using assms(2) by auto
+    have fins: "finite (J \<inter> I)" "finite (I - J)" using fin_I by auto
     have b: "I = (J \<inter> I) \<union> (I - J)" by auto
-    let ?q1 = "Pi_pmf (J \<inter> I) d p"
-    let ?q2 = "Pi_pmf (I - J) d p"
+    let ?q1 = "Pi_pmf (J \<inter> I) d M"
+    let ?q2 = "Pi_pmf (I - J) d M"
     let ?c = "(\<lambda>(x,y) i. if i \<in> (J \<inter> I) then x i else y i)"
-    let ?c1 = "(\<lambda>x i. if i \<in> (J \<inter> I) then x i else d)"
-    let ?c2 = "(\<lambda>x i. if i \<in> (I - J) then x i else d)"
+    let ?c1 = "(\<lambda>x i. if i \<in> (J \<inter> I) then x i else \<delta> i)"
+    let ?c2 = "(\<lambda>x i. if i \<in> (I - J) then x i else \<delta> i)"
+    let ?v = "fst \<omega>"
+    let ?w = "snd \<omega>"
 
-    have c:"?runr m (?c (x,y)) = fst \<omega> \<longleftrightarrow> ?runr m x = fst \<omega>" if "(x,y) \<in> set_pmf (pair_pmf ?q1 ?q2)" for x y
+    have c_space: "?c (x, y) \<in> set_pmf space" if "x \<in> set_pmf ?q1" and "y \<in> set_pmf ?q2" for x y
+      using that unfolding space_def set_Pi_pmf[OF fin_I] set_Pi_pmf[OF fins(1)]
+        set_Pi_pmf[OF fins(2)] by (auto simp:PiE_dflt_def)
+
+    have c:"?r m (?c (x,y)) = fst \<omega> \<longleftrightarrow> ?r m (?c1 x) = fst \<omega>"
+      if "(x,y) \<in> set_pmf (pair_pmf ?q1 ?q2)" for x y
     proof -
-      have "\<And>i. i \<notin> J \<inter> I \<Longrightarrow> x i = d" "\<And>i. i \<notin> I - J \<Longrightarrow> y i = d"
-        using that unfolding set_pair_pmf set_Pi_pmf[OF fins(1)]  set_Pi_pmf[OF fins(2)] PiE_dflt_def by force+
-      hence cd:"?runr (map_rd ((=) (fst \<omega>)) m) (?c (x,y)) = ?runr (map_rd ((=) (fst \<omega>)) m) x"
-        by (intro depends_onD[OF J_dep(1)]) auto
-      hence "?runr m (?c (x,y)) = fst \<omega> \<longleftrightarrow> ?runr (map_rd ((=) (fst \<omega>)) m) x = True"
+      have "?r (map_rd ((=) (fst \<omega>)) m) (?c (x,y)) = ?r (map_rd ((=) (fst \<omega>)) m) (?c1 x)"
+        using that by (intro depends_onD[OF J_dep(1)] c_space 1) auto
+      hence "?r m (?c (x,y)) = fst \<omega> \<longleftrightarrow> ?r (map_rd ((=) (fst \<omega>)) m) (?c1 x) = True"
         by (auto simp: run_reader_simps)
-      also have "... \<longleftrightarrow>  ?runr m x = fst \<omega>" by (auto simp: run_reader_simps)
+      also have "... \<longleftrightarrow>  ?r m (?c1 x) = fst \<omega>" by (auto simp: run_reader_simps)
       finally show ?thesis by simp
     qed
 
-    have d: "?runr (f (fst \<omega>)) (?c (x,y)) = ?runr (f (fst \<omega>)) y"  for x y
-      by (intro depends_onD[OF J_dep(2)]) auto
+    have d: "?r (f (fst \<omega>)) (?c (x,y)) = ?r (f (fst \<omega>)) (?c2 y)"
+      if "(x,y) \<in> set_pmf (pair_pmf ?q1 ?q2)" for x y using that
+      by (intro depends_onD[OF J_dep(2)] 1 c_space) (simp_all add:restrict_def cong:if_cong)
 
-    have e:"?runr m (?c1 x) = fst \<omega> \<longleftrightarrow> ?runr m x = fst \<omega>" if "(x,y) \<in> set_pmf (pair_pmf q q)" for x y
+    have e:"?r m (?c1 x) = fst \<omega> \<longleftrightarrow> ?r m x = fst \<omega>"
+      if "(x,y) \<in> set_pmf (pair_pmf space space)" for x y
     proof -
-      have "\<And>i. i \<notin> I \<Longrightarrow> x i = d" "\<And>i. i \<notin> I \<Longrightarrow> y i = d"
-        using that unfolding set_pair_pmf q_def set_Pi_pmf[OF assms(2)] PiE_dflt_def by force+
-      hence cd:"?runr (map_rd ((=) (fst \<omega>)) m) (?c1 x) = ?runr (map_rd ((=) (fst \<omega>)) m) x"
-        by (intro depends_onD[OF J_dep(1)]) auto
-      hence "?runr m (?c1 x) = fst \<omega> \<longleftrightarrow> ?runr (map_rd ((=) (fst \<omega>)) m) x = True"
+      have "?r (map_rd ((=) (fst \<omega>)) m) (?c1 x) = ?r (map_rd ((=) (fst \<omega>)) m) x" using that
+        by (intro depends_onD[OF J_dep(1)] 2) (simp_all add:space_def restrict_def cong:if_cong)
+      hence "?r m (?c1 x) = fst \<omega> \<longleftrightarrow> ?r (map_rd ((=) (fst \<omega>)) m) x = True"
         by (auto simp: run_reader_simps)
-      also have "... \<longleftrightarrow>  ?runr m x = fst \<omega>" by (auto simp: run_reader_simps)
+      also have "\<dots> \<longleftrightarrow> ?r m x = fst \<omega>" by (auto simp: run_reader_simps)
       finally show ?thesis by simp
     qed
 
-    have f: "?runr (f (fst \<omega>)) (?c2 y) = ?runr (f (fst \<omega>)) y" if "(x,y) \<in> set_pmf (pair_pmf q q)" for x y
-    proof -
-      have  "\<And>i. i \<notin> I \<Longrightarrow> y i = d"
-        using that unfolding q_def set_Pi_pmf[OF assms(2)] set_pair_pmf PiE_dflt_def by simp
-      thus ?thesis
-        by (intro depends_onD[OF J_dep(2)]) auto
-    qed
+    have f: "?r (f (fst \<omega>)) (?c2 y) = ?r (f (fst \<omega>)) y" if "(x,y) \<in> set_pmf (pair_pmf space space)"
+      for x y using that
+      by (intro depends_onD[OF J_dep(2)] 2) (simp_all add:space_def restrict_def cong:if_cong)
 
-    have "pmf ?L1 \<omega> = measure_pmf.prob q {x. (run_reader m x, run_reader (f (run_reader m x)) x) = \<omega>}"
+    have "pmf ?L1 \<omega> = measure space {x. (run_reader m x, run_reader (f (run_reader m x)) x) = \<omega>}"
       unfolding pmf_map by (simp add:Let_def vimage_def)
-    also have "... = measure (Pi_pmf ((J \<inter> I) \<union> (I-J)) d p) {x. ?runr m x = fst \<omega> \<and> ?runr (f (fst \<omega>)) x = snd \<omega>}"
-      unfolding q_def by (intro arg_cong2[where f="measure_pmf.prob"] arg_cong[where f="\<lambda>I. Pi_pmf I d p"]) auto
-    also have "... = measure (map_pmf ?c (pair_pmf ?q1 ?q2)) {x. ?runr m x = fst \<omega> \<and> ?runr (f (fst \<omega>)) x = snd \<omega>}"
-      using assms(2) by (intro arg_cong2[where f="measure_pmf.prob"] Pi_pmf_union) auto
-    also have "... = measure (pair_pmf ?q1 ?q2) {(x,y). ?runr m (?c (x,y))=fst \<omega> \<and> ?runr (f (fst \<omega>)) (?c (x,y))=snd \<omega>}"
+    also have "\<dots> = measure (Pi_pmf ((J\<inter>I) \<union> (I-J)) d M) {x. ?r m x = ?v \<and> ?r (f (fst \<omega>)) x = ?w}"
+      unfolding space_def
+      by (intro arg_cong2[where f="measure_pmf.prob"] arg_cong[where f="\<lambda>I. Pi_pmf I d M"]) auto
+    also have "\<dots> = measure (map_pmf ?c (pair_pmf ?q1 ?q2)) {x. ?r m x=?v \<and> ?r (f (fst \<omega>)) x=?w}"
+      using fin_I by (intro arg_cong2[where f="measure_pmf.prob"] Pi_pmf_union) auto
+    also have "\<dots> = measure (pair_pmf ?q1 ?q2) {(x,y). ?r m (?c (x,y))=?v\<and>?r (f ?v) (?c (x,y))=?w}"
       by (simp add:case_prod_beta' cong:if_cong)
-    also have "... = measure (pair_pmf ?q1 ?q2) {(x,y). ?runr m x = fst \<omega> \<and> ?runr (f (fst \<omega>)) y = snd \<omega>}"
+    also have "\<dots> = measure (pair_pmf ?q1 ?q2) {(x,y). ?r m (?c1 x) = ?v \<and> ?r (f ?v) (?c2 y) = ?w}"
       using c d by (intro measure_pmf_cong) auto
-    also have "... = measure(pair_pmf(map_pmf ?c1 q)(map_pmf ?c2 q)){(x,y). ?runr m x=fst \<omega>\<and>?runr(f(fst \<omega>))y=snd \<omega>}"
-      unfolding q_def using assms(2)
-      by (intro arg_cong2[where f="measure_pmf.prob"] arg_cong2[where f="pair_pmf"] Pi_pmf_subset) auto
-    also have "... = measure (pair_pmf q q) {(x,y). ?runr m (?c1 x) = fst \<omega> \<and> ?runr (f (fst \<omega>)) (?c2 y) = snd \<omega>}"
-      by (simp add:map_pair[symmetric] case_prod_beta' cong:if_cong)
-    also have "... = measure (pair_pmf q q) {(x,y). ?runr m x = fst \<omega> \<and> ?runr (f (fst \<omega>)) y = snd \<omega>}"
+    also have "\<dots> = measure (pair_pmf
+      (map_pmf (\<lambda>f. restrict_dfl f (J \<inter> I) d) space) (map_pmf (\<lambda>f. restrict_dfl f (I-J) d) space))
+      {(x,y). ?r m (?c1 x)=?v\<and>?r(f ?v) (?c2 y)=?w}"
+      unfolding space_def restrict_dfl_def using fin_I by (intro arg_cong2[where f="pair_pmf"]
+          arg_cong2[where f="measure_pmf.prob"] Pi_pmf_subset) auto
+    also have "\<dots> = measure (pair_pmf space space) {(x,y). ?r m (?c1 x)=?v \<and> ?r (f ?v) (?c2 y)=?w}"
+      by (simp add: restrict_dfl_def map_pair[symmetric] case_prod_beta' cong:if_cong)
+    also have "\<dots> = measure (pair_pmf space space) {(x,y). ?r m x = ?v \<and> ?r (f ?v) y = ?w}"
       using e f by (intro measure_pmf_cong) auto
-    also have "... = (\<integral>x. measure (map_pmf (Pair x) q) {(x,y). ?runr m x = fst \<omega> \<and> ?runr (f (fst \<omega>)) y = snd \<omega>} \<partial>q)"
+    also have "\<dots> = (\<integral>x. measure (map_pmf (Pair x) space) {(x,y). ?r m x=?v\<and>?r(f ?v) y=?w} \<partial>space)"
       unfolding pair_pmf_def by (subst measure_bind_pmf) (simp add:map_pmf_def)
-    also have "... = (\<integral>x. measure q {y. ?runr m x = fst \<omega> \<and> ?runr (f (fst \<omega>)) y = snd \<omega>} \<partial>q)"
+    also have "\<dots> = (\<integral>x. measure space {y. ?r m x = fst \<omega> \<and> ?r (f (fst \<omega>)) y = snd \<omega>} \<partial>space)"
       by (intro integral_cong_AE) simp_all
-    also have "... = (\<integral>x. measure q {y. (run_reader m x, run_reader (f (run_reader m x)) y) = \<omega>} \<partial>q)"
+    also have "\<dots> = (\<integral>x. measure space {y. (?r m x, ?r (f (?r m x)) y) = \<omega>} \<partial>space)"
       by (intro integral_cong_AE AE_pmfI measure_pmf_cong) auto
-    also have "... = pmf ?R1 \<omega>" unfolding pmf_bind pmf_map vimage_def by simp
+    also have "\<dots> = pmf ?R1 \<omega>" unfolding pmf_bind pmf_map vimage_def sample_def by simp
     finally show "pmf ?L1 \<omega> = pmf ?R1 \<omega>" by simp
   qed
 
-  have "?L = map_pmf snd (map_pmf (\<lambda>\<phi>. let v = run_reader m \<phi> in (v,run_reader (f v) \<phi>)) q)"
-    unfolding map_pmf_comp by (intro map_pmf_cong refl) (simp add:run_reader_simps Let_def)
-  also have "... = map_pmf snd (bind_pmf (?run m) (\<lambda>v. map_pmf (Pair v) (?run (f v))))"
+  have "?L = map_pmf snd (map_pmf (\<lambda>\<phi>. let v = run_reader m \<phi> in (v,run_reader (f v) \<phi>)) space)"
+    unfolding map_pmf_comp sample_def
+    by (intro map_pmf_cong refl) (simp add:run_reader_simps Let_def)
+  also have "\<dots> = map_pmf snd (bind_pmf (sample m) (\<lambda>v. map_pmf (Pair v) (sample (f v))))"
     unfolding a by simp
-  also have "... = ?R"
+  also have "\<dots> = ?R"
     unfolding map_bind_pmf by (simp add:map_pmf_comp)
   finally show ?thesis
     by simp
 qed
 
 lemma lazify_return:
-  "map_pmf (run_reader (return_rd x)) p = return_pmf x" (is "?L = ?R")
+  "sample (return_rd x) = return_pmf x" (is "?L = ?R")
 proof -
-  have "?L = map_pmf (\<lambda>_. x) p" by (intro map_pmf_cong refl) (simp add:run_reader_simps)
+  have "?L = map_pmf (\<lambda>_. x) space" unfolding sample_def
+    by (intro map_pmf_cong refl) (simp add:run_reader_simps)
   also have "... = ?R" by simp
   finally show ?thesis by simp
 qed
 
 lemma lazify_bind_return:
-  assumes "finite I"
-  shows
-  "map_pmf (run_reader (bind_rd m (\<lambda>x. return_rd (f x)))) (Pi_pmf I d p) =
-    map_pmf (run_reader m) (Pi_pmf I d p) \<bind> (\<lambda>x. return_pmf (f x))" (is "?L = ?R")
+  "sample (bind_rd m (\<lambda>x. return_rd (f x))) = sample m \<bind> (\<lambda>x. return_pmf (f x))" (is "?L = ?R")
 proof -
-  have "?L = map_pmf (run_reader m) (Pi_pmf I d p) \<bind> (\<lambda>x. map_pmf (run_reader (return_rd (f x))) (Pi_pmf I d p))"
-    by (intro assms lazify_bind independent_bindI[where F="(\<lambda>_. UNIV)"] depends_on_univ conjI depends_on_return)
+  have "?L = sample m \<bind> (\<lambda>v. sample (return_rd (f v)))"
+    by (intro lazify_bind independent_bindI[where F="(\<lambda>_. UNIV)"]
+        depends_on_univ conjI depends_on_return)
   also have "... = ?R"
     unfolding lazify_return by simp
   finally show ?thesis by simp
 qed
+
+end
 
 end
